# baseURI : http://example.org/issda

@prefix issda: <http://example.org/issda#> .
@prefix owl: <http://www.w3.org/2002/07/owl#> .
@prefix rdf: <http://www.w3.org/1999/02/22-rdf-syntax-ns#> .
@prefix rdfs: <http://www.w3.org/2000/01/rdf-schema#> .
@prefix xsd: <http://www.w3.org/2001/XMLSchema#> .

# Classes and their subclasses

# Class MeterId and its subclasses 

issda:MeterId
  rdf:type owl:Class .

issda:ResidentialMeter
  rdfs:subClassOf issda:MeterId .

issda:SmeMeter
  rdfs:subClassOf issda:MeterId .

# Class Building and its subclasses

issda:Building
  rdf:type owl:Class.

issda:ResidentialBuilding
  rdfs:subClassOf issda:Building .

issda:ProfessionalBuilding
  rdfs:subClassOf issda:Building .

issda:Apartment 
  rdfs:subClassOf issda:ResidentialBuilding .

issda:SemiDetachedHouse
  rdfs:subClassOf issda:ResidentialBuilding .

issda:DetachedHouse
  rdfs:subClassOf issda:ResidentialBuilding .

issda:TerracedHouse
  rdfs:subClassOf issda:ResidentialBuilding .

issda:Bungalow
  rdfs:subClassOf issda:ResidentialBuilding .

# Class Occupier and its subclasses

issda:Occupier
  rdf:type owl:Class .

issda:Household
  rdfs:subClassOf issda:Occupier .

issda:Organization
  rdfs:subClassOf issda:Occupier .

# Class BusinessCategory and its instances

issda:BusinessCategory
   rdf:type owl:Class .

issda:agriculture
   rdf:type issda:BusinessCategory;
   rdfs:label "Agriculture, forestry and fishing" .

issda:industry
   rdf:type issda:BusinessCategory;
   rdfs:label "Industry Mining and quarrying Manufacturing Electricity, gas, steam and air conditioning supply Water supply, sewerage, waste management and remediation activities" .

issda:construction
   rdf:type issda:BusinessCategory;
   rdfs:label "Construction" .

issda:tradeOrRepair
   rdf:type issda:BusinessCategory;
   rdfs:label "Wholesale and retail trade; repair of motor vehicles and motorcycles" .

issda:businessOrService
   rdf:type issda:BusinessCategory;
   rdfs:label "Business and Professional Services Information and communication Financial and insurance activities Real estate activities Professional, scientific and technical activities Administrative and support service activities Public administration and defence; compulsory social security Education Human health and social work activities" .

issda:transportationOrStorageOrAccomodation
   rdf:type issda:BusinessCategory;
   rdfs:label "Other Transportation and storage Accommodation and food service activities Leisure hotels Arts, entertainment and recreation Other service activities Activities of households as employers; undifferentiated goods- and services producing activities of households for own use Activities of extra-territorial organisations and bodies" .


# Properties of domain Meter or its subclasses

issda:consumption
  rdf:type owl:DynamicProperty ;
  rdfs:domain issda:MeterId ;
  rdfs:range xsd:integer ;
rdfs:comment "dynamic property that associates the consumption to a meter at different timestamps" .

issda:timestamp rdfs:range xsd:dateTime .

issda:associatedOccupier 
  rdf:type owl:ObjectProperty ;
  rdfs:domain issda:MeterId ;
  rdfs:range issda:Occupier ;
rdfs:comment "Expresses the relation from a meter number to an occupier" .

issda:associatedBuilding 
  rdf:type owl:ObjectProperty ;
  rdfs:domain issda:MeterId ;
  rdfs:range issda:Building ;
rdfs:comment "Expresses the relation from a meter to a building" .

issda:broadbandInternet
  rdf:type owl:DatatypeProperty ;
  rdfs:domain issda:MeterId ;
  rdfs:range xsd:boolean ;
rdfs:comment "Expresses the boolean property for a meter to have a broadband internet connection" .

issda:narrowbandInternet
  rdf:type owl:DatatypeProperty ;
  rdfs:domain issda:MeterId ;
  rdfs:range xsd:boolean ;
rdfs:comment "Expresses the boolean property for a meter to have a narrowband internet connection" .

issda:broadbandInternet
   rdfs:subPropertyOf issda:internet .

issda:narrowbandInternet
   rdfs:subPropertyOf issda:internet .
   
For meters id without internet connection, add the triples id issda:internet "false"
   
# Properties of domain Occupier or its subclasses

issda:rent
  rdf:type owl:ObjectProperty ;
  rdfs:domain issda:Occupier ;
  rdfs:range issda:Building ;
rdfs:comment "Expresses the renting relation between an occupier and a building" .

issda:owns
  rdf:type owl:ObjectProperty ;
  rdfs:domain issda:Occupier ;
  rdfs:range issda:Building ;
rdfs:comment "Expresses the owning relation between an occupier and a building" .

issda:numberUnderFifteen
  rdf:type owl:DatatypeProperty ;
  rdfs:domain issda:Occupier ;
  rdfs:range xsd:integer ; 
  rdfs:comment "Number of persons under fifteen in the home. Maybe zero if only one person in the home" .

issda:numberOverFifteen
  rdf:type owl:DatatypeProperty ;
  rdfs:domain issda:Occupier ;
  rdfs:range xsd:integer ;
  rdfs:comment "Number of persons over fifteen in the home, including the contract holder".

issda:numberOfPersons
  rdf:type owl:DatatypeProperty ;
  rdfs:domain issda:Occupier ;  
  rdfs:range xsd:integer ;
 rdfs:comment "Expresses the number of persons at home using integer value such as 1, 2, 3 and 5.
  
issda:familySize
  rdf:type owl:DatatypeProperty ;
  rdfs:domain issda:Occupier ;  
  rdfs:range xsd:string ;
  rdfs:comment "Expresses the number of persons at home using the predefined string values: Small (family of 1-3 persons), Medium (family of 3-5 persons) and Large (family of more than 6 persons)".
  
issda:chiefIncomeEarnerEducation
  rdf:type owl:DatatypeProperty ;  
  rdfs:domain issda:Household ;
  rdfs:range xsd:string;
  rdfs:comment "Expresses the last diploma attained by chief income earner using the string values".

issda:chiefIncomeEarnerEducationLevel
  rdf:type owl:DatatypeProperty ;  
  rdfs:domain issda:Household ;
  rdfs:range xsd:string;
  rdfs:comment "Expresses the level of education of the chief income earner using the predefined string values: noFormalEducation, primary, secondaryToJuniorCertLevel, secondaryToLeavingCertLevel, third" .  

issda:yearlyIncome
  rdf:type owl:DatatypeProperty ; 
  rdfs:domain issda:Occupier ;
  rdfs:range xsd:integer;
rdfs:comment "Expresses the exact yearly income of occupier in Euros using integer values such as 5000, 25000 and 75000".

issda:yearlyIncomeRange
  rdf:type owl:DatatypeProperty ; 
  rdfs:domain issda:Occupier ;
  rdfs:range xsd:string;
rdfs:comment "Expresses the yearly income in Euros using the predefined string values: Low (less than 25000), Average (between 25000-75000), High (more than 75000)".

issda:chiefIncomeEarnerStatus 
  rdfs:domain issda:Household ;
  rdfs:range xsd:string;
rdfs:comment "Expresses the employment status of the chief income earner using the predefined string values: employee, selfEmployed, unemployed, retired, carer" .

issda:business
  rdfs:domain issda:Organization ;
  rdfs:range issda:BusinessCategory;
rdfs:comment "Expresses the business of the organization: one of the instances of the class BusinessCategory" .

issda:numberOfEmployees
  rdf:type owl:DatatypeProperty ;
  rdfs:domain issda:Organization;
  rdfs:range xsd:string ;
rdfs:comment "Expresses the number of employees in an organization using the predefined string values: soleEmpoyee, between 1-5, between 6-10, between 11-24, between 25-49, between 50-99, between100-199, more than 200 " .

issda:yearlyTurnover
  rdf:type owl:DatatypeProperty ;
  rdfs:domain issda:Organization ;
  rdfs:range xsd:string;
rdfs:comment "Expresses the yearly turnover of the organization in Euros using the predefined string values: less than 58000, between 59000-100000, between 101000-250000, between 251000-500000, between 501000-750000, between 751000-1M, between 1M-1.5M, between 1.6M-2M, between 3M-5M, between 6M-10M, between 11M-20M, more than 20M " .

# Properties of domain Building or its subclasses

issda:buildingAge 
  rdf:type owl:DatatypeProperty ;
  rdfs:domain issda:Building ;
  rdfs:range xsd:integer;
rdfs:comment "Expresses the exact age of building in years using integer values such as 5, 10 and 25".

issda:buildingAgeRange 
  rdf:type owl:DatatypeProperty ;
  rdfs:domain issda:Building ;
  rdfs:range xsd:string;
rdfs:comment "Expresses the age of a building using predefined string values: New (less than 5years), Between new and old (between 5-20years), Old (more than 25years)".

issda:surfaceArea
  rdf:type owl:DatatypeProperty ;
  rdfs:domain issda:Building;
  rdfs:range xsd:integer ;
rdfs:comment "Expresses the surface of a building in square meters using integer values such as 500, 750 and 1000".

issda:numberOfBedrooms
  rdf:type owl:DatatypeProperty ;
  rdfs:domain issda:ResidentialBuilding ;
  rdfs:range xsd:integer ;
rdfs:comment "Expresses the number of bedrooms of a residential building using integer values such as 1, 2, 3 and 4."

issda:heatingEnergySource 
  rdf:type owl:DatatypeProperty ;
  rdfs:domain issda:ResidentialBuilding ;
  rdfs:range xsd:string;
rdfs:comment "Expresses the heating of a residential building using predefined string values: electric, gas, oil, solidFuel, renewable" .

issda:waterHeatingEnergySource 
  rdf:type owl:DatatypeProperty ;
  rdfs:domain issda:ResidentialBuilding ;
  rdfs:range xsd:string;
rdfs:comment "Expresses the water heating of a residential building using predefined string values: centralHeatingSystem, electric, gas, oil, solidFuel, renewable" .
 
issda:cookingEnergySource rdf:type owl:DatatypeProperty ;
  rdfs:domain issda:ResidentialBuilding ;
  rdfs:range xsd:string;
rdfs:comment "Expresses the cooking energy of a residential building using predefined string values: electric, gas, oil, solidFuel" .

issda:heatingEnergySource 
   rdfs:subPropertyOf issda:buildingEnergySource .

issda:waterHeatingEnergySource 
   rdfs:subPropertyOf issda:buildingEnergySource .

issda:cookingEnergySource 
   rdfs:subPropertyOf issda:buildingEnergySource .

issda:numberOfWashingMachine 
  rdf:type owl:DatatypeProperty ;
  rdfs:domain issda:ResidentialBuilding ;
  rdfs:range xsd:integer .

issda:numberOfTumbleDryer
  rdf:type owl:DatatypeProperty ;
  rdfs:domain issda:ResidentialBuilding ;
  rdfs:range xsd:integer .

issda:numberOfDishWasher
  rdf:type owl:DatatypeProperty ;
  rdfs:domain issda:ResidentialBuilding ;
  rdfs:range xsd:integer .

issda:numberOfElectricCooker
  rdf:type owl:DatatypeProperty ;
  rdfs:domain issda:ResidentialBuilding ;
  rdfs:range xsd:integer .

issda:numberOfFreezer
  rdf:type owl:DatatypeProperty ;
  rdfs:domain issda:ResidentialBuilding ;
  rdfs:range xsd:integer .

issda:numberOfTV
  rdf:type owl:DatatypeProperty ;
  rdfs:domain issda:ResidentialBuilding ;
  rdfs:range xsd:integer .

issda:numberOfComputer
  rdf:type owl:DatatypeProperty ;
  rdfs:domain issda:ResidentialBuilding ;
  rdfs:range xsd:integer .

issda:numberOfGameConsole
  rdf:type owl:DatatypeProperty ;
  rdfs:domain issda:ResidentialBuilding ;
  rdfs:range xsd:integer.

issda:atticInsulated
  rdf:type owl:DatatypeProperty ;
  rdfs:domain issda:ResidentialBuilding ;
  rdfs:range xsd:boolean ;
rdfs:comment "Expresses the boolean property for a residential building to have its attic insulated" .

issda:externalWallInsulated
  rdf:type owl:DatatypeProperty ;
  rdfs:domain issda:Building ;
  rdfs:range xsd:boolean ;
rdfs:comment "Expresses the boolean property for a building to have its external walls insulated" .

issda:electricCoolingAppliance
  rdf:type owl:DatatypeProperty ;
  rdfs:domain issda:ProfessionalBuilding ;
  rdfs:range xsd:boolean . 

issda:electricHeatingAppliance
  rdf:type owl:DatatypeProperty ;
  rdfs:domain issda:ProfessionalBuilding ;
  rdfs:range xsd:boolean .

issda:electricLightingAppliance
  rdf:type owl:DatatypeProperty ;
  rdfs:domain issda:ProfessionalBuilding ;
  rdfs:range xsd:boolean .

issda:electricOfficeEquipment
  rdf:type owl:DatatypeProperty ;
  rdfs:domain issda:ProfessionalBuilding ;
  rdfs:range xsd:boolean .

issda:electricManufacturingEquipment
  rdf:type owl:DatatypeProperty ;
  rdfs:domain issda:ProfessionalBuilding ;
  rdfs:range xsd:boolean .

issda:electricEquipment
  rdf:type owl:DatatypeProperty ;
  rdfs:domain issda:ProfessionalBuilding ;
  rdfs:range xsd:boolean .

issda:electricCoolingAppliance
  rdfs:subPropertyOf issda:electricEquipment .

issda:electricHeatingAppliance
  rdfs:subPropertyOf issda:electricEquipment .

issda:electricLightingAppliance
  rdfs:subPropertyOf issda:electricEquipment .

issda:electricOfficeEquipment
  rdfs:subPropertyOf issda:electricEquipment .

issda:electricManufacturingEquipment
  rdfs:subPropertyOf issda:electricEquipment .
